mls

bedrock2/src/bedrock2/MetricLeakageSemantics.v
@@ -14,6 +14,11 @@ Require Import Coq.Lists.List.
 
 Local Notation UNK := String.EmptyString.
 
+Inductive AEP :=
+| AEP_A : (nat -> AEP) -> AEP
+| AEP_E : (nat -> AEP) -> AEP
+| AEP_P : Prop -> AEP.
+
 Section semantics.
   Context {width: Z} {BW: Bitwidth width} {word: word.word width} {mem: map.map word byte}.
   Context {locals: map.map String.string word}.
@@ -76,105 +81,114 @@ Module exec. Section WithParams.
 
   Local Notation metrics := MetricLog.
 
-  Implicit Types post : leakage -> trace -> mem -> locals -> metrics -> Prop. (* COQBUG: unification finds Type instead of Prop and fails to downgrade *)
+  Implicit Types post : bool -> AEP -> leakage -> trace -> mem -> locals -> metrics -> Prop. (* COQBUG: unification finds Type instead of Prop and fails to downgrade *)
   Inductive exec {pick_sp: PickSp} :
-    cmd -> leakage -> trace -> mem -> locals -> metrics ->
-    (leakage -> trace -> mem -> locals -> metrics -> Prop) -> Prop :=
+    cmd -> bool -> AEP -> leakage -> trace -> mem -> locals -> metrics ->
+    (bool -> AEP -> leakage -> trace -> mem -> locals -> metrics -> Prop) -> Prop :=
   | skip
-    k t m l mc post
-    (_ : post k t m l mc)
-    : exec cmd.skip k t m l mc post
+    aep k t m l mc post
+    (_ : post true aep k t m l mc)
+    : exec cmd.skip true aep k t m l mc post
   | set x e
-    k t m l mc post
+    aep k t m l mc post
     v k' mc' (_ : eval_expr m l e k mc = Some (v, k', mc'))
-    (_ : post k' t m (map.put l x v) (cost_set isRegStr x UNK mc'))
-    : exec (cmd.set x e) k t m l mc post
+    (_ : post true aep k' t m (map.put l x v) (cost_set isRegStr x UNK mc'))
+    : exec (cmd.set x e) true aep k t m l mc post
   | unset x
-    k t m l mc post
-    (_ : post k t m (map.remove l x) mc)
-    : exec (cmd.unset x) k t m l mc post
+    aep k t m l mc post
+    (_ : post true aep k t m (map.remove l x) mc)
+    : exec (cmd.unset x) true aep k t m l mc post
   | store sz ea ev
-    k t m l mc post
+    aep k t m l mc post
     a k' mc' (_ : eval_expr m l ea k mc = Some (a, k', mc'))
     v k'' mc'' (_ : eval_expr m l ev k' mc' = Some (v, k'', mc''))
     m' (_ : store sz m a v = Some m')
-    (_ : post (leak_word a :: k'') t m' l (cost_store isRegStr UNK UNK mc''))
-    : exec (cmd.store sz ea ev) k t m l mc post
+    (_ : post true aep (leak_word a :: k'') t m' l (cost_store isRegStr UNK UNK mc''))
+    : exec (cmd.store sz ea ev) true aep k t m l mc post
   | stackalloc x n body
-    k t mSmall l mc post
+    aep k t mSmall l mc post
     (_ : Z.modulo n (bytes_per_word width) = 0)
     (_ : forall mStack mCombined,
         let a := pick_sp k in
         anybytes a n mStack ->
         map.split mCombined mSmall mStack ->
-        exec body (leak_unit :: k) t mCombined (map.put l x a) (cost_stackalloc isRegStr x mc)
-          (fun k' t' mCombined' l' mc' =>
+        exec body true aep (leak_unit :: k) t mCombined (map.put l x a) (cost_stackalloc isRegStr x mc)
+          (fun q' aep' k' t' mCombined' l' mc' =>
             exists mSmall' mStack',
               anybytes a n mStack' /\
               map.split mCombined' mSmall' mStack' /\
-              post k' t' mSmall' l' mc'))
-     : exec (cmd.stackalloc x n body) k t mSmall l mc post
-  | if_true k t m l mc e c1 c2 post
+              post q' aep' k' t' mSmall' l' mc'))
+     : exec (cmd.stackalloc x n body) true aep k t mSmall l mc post
+  | if_true aep k t m l mc e c1 c2 post
     v k' mc' (_ : eval_expr m l e k mc = Some (v, k', mc'))
     (_ : word.unsigned v <> 0)
-    (_ : exec c1 (leak_bool true :: k') t m l (cost_if isRegStr UNK (Some UNK) mc') post)
-    : exec (cmd.cond e c1 c2) k t m l mc post
+    (_ : exec c1 true aep (leak_bool true :: k') t m l (cost_if isRegStr UNK (Some UNK) mc') post)
+    : exec (cmd.cond e c1 c2) true aep k t m l mc post
   | if_false e c1 c2
-    k t m l mc post
+    aep k t m l mc post
     v k' mc' (_ : eval_expr m l e k mc = Some (v, k', mc'))
     (_ : word.unsigned v = 0)
-    (_ : exec c2 (leak_bool false :: k') t m l (cost_if isRegStr UNK (Some UNK) mc') post)
-    : exec (cmd.cond e c1 c2) k t m l mc post
+    (_ : exec c2 true aep (leak_bool false :: k') t m l (cost_if isRegStr UNK (Some UNK) mc') post)
+    : exec (cmd.cond e c1 c2) true aep k t m l mc post
   | seq c1 c2
-    k t m l mc post
-    mid (_ : exec c1 k t m l mc mid)
-    (_ : forall k' t' m' l' mc', mid k' t' m' l' mc' -> exec c2 k' t' m' l' mc' post)
-    : exec (cmd.seq c1 c2) k t m l mc post
+    aep k t m l mc post
+    mid (_ : exec c1 true aep k t m l mc mid)
+    (_ : forall q' aep' k' t' m' l' mc', mid q' aep' k' t' m' l' mc' -> exec c2 q' aep' k' t' m' l' mc' post)
+    : exec (cmd.seq c1 c2) true aep k t m l mc post
   | while_false e c
-    k t m l mc post
+    aep k t m l mc post
     v k' mc' (_ : eval_expr m l e k mc = Some (v, k', mc'))
     (_ : word.unsigned v = 0)
-    (_ : post (leak_bool false :: k') t m l (cost_loop_false isRegStr UNK (Some UNK) mc'))
-    : exec (cmd.while e c) k t m l mc post
+    (_ : post true aep (leak_bool false :: k') t m l (cost_loop_false isRegStr UNK (Some UNK) mc'))
+    : exec (cmd.while e c) true aep k t m l mc post
   | while_true e c
-      k t m l mc post
+      aep k t m l mc post
       v k' mc' (_ : eval_expr m l e k mc = Some (v, k', mc'))
       (_ : word.unsigned v <> 0)
-      mid (_ : exec c (leak_bool true :: k') t m l mc' mid)
-      (_ : forall k'' t' m' l' mc'', mid k'' t' m' l' mc'' ->
-                                 exec (cmd.while e c) k'' t' m' l' (cost_loop_true isRegStr UNK (Some UNK) mc'') post)
-    : exec (cmd.while e c) k t m l mc post
+      mid (_ : exec c true aep (leak_bool true :: k') t m l mc' mid)
+      (_ : forall q' aep' k'' t' m' l' mc'', mid q' aep' k'' t' m' l' mc'' ->
+                                 exec (cmd.while e c) q' aep' k'' t' m' l' (cost_loop_true isRegStr UNK (Some UNK) mc'') post)
+    : exec (cmd.while e c) true aep k t m l mc post
   | call binds fname arges
-      k t m l mc post
+      aep k t m l mc post
       params rets fbody (_ : map.get e fname = Some (params, rets, fbody))
       args k' mc' (_ : eval_call_args m l arges k mc = Some (args, k', mc'))
       lf (_ : map.of_list_zip params args = Some lf)
-      mid (_ : exec fbody (leak_unit :: k') t m lf mc' mid)
-      (_ : forall k'' t' m' st1 mc'', mid k'' t' m' st1 mc'' ->
+      mid (_ : exec fbody true aep (leak_unit :: k') t m lf mc' mid)
+      (_ : forall q' aep' k'' t' m' st1 mc'', mid q' aep' k'' t' m' st1 mc'' ->
           exists retvs, map.getmany_of_list st1 rets = Some retvs /\
           exists l', map.putmany_of_list_zip binds retvs l = Some l' /\
-          post k'' t' m' l'  (cost_call PreSpill mc''))
-    : exec (cmd.call binds fname arges) k t m l mc post
+          post q' aep' k'' t' m' l'  (cost_call PreSpill mc''))
+    : exec (cmd.call binds fname arges) true aep k t m l mc post
   | interact binds action arges
-      k t m l mc post
+      aep k t m l mc post
       mKeep mGive (_: map.split m mKeep mGive)
       args k' mc' (_ :  eval_call_args m l arges k mc = Some (args, k', mc'))
       mid (_ : ext_spec t mGive action args mid)
       (_ : forall mReceive resvals klist, mid mReceive resvals klist ->
           exists l', map.putmany_of_list_zip binds resvals l = Some l' /\
           forall m', map.split m' mKeep mReceive ->
-          post (leak_list klist :: k') (cons ((mGive, action, args), (mReceive, resvals)) t) m' l'
+          post true aep (leak_list klist :: k') (cons ((mGive, action, args), (mReceive, resvals)) t) m' l'
             (cost_interact PreSpill mc'))
-    : exec (cmd.interact binds action arges) k t m l mc post
+    : exec (cmd.interact binds action arges) true aep k t m l mc post
+  | quit s q aep k t m l mc post
+      (_ : post false aep k t m l mc)
+    : exec s q aep k t m l mc post
+  | exec_A s q aep k t m l mc post
+      (_ : forall x, exec s q (aep x) k t m l mc post)
+    : exec s q (AEP_A aep) k t m l mc post
+  | exec_E s q aep k t m l mc post x
+      (_ : exec s q (aep x) k t m l mc post)
+    : exec s q (AEP_E aep) k t m l mc post
   .
 
   Context {word_ok: word.ok word} {mem_ok: map.ok mem} {ext_spec_ok: ext_spec.ok ext_spec}.
 
-  Lemma weaken {pick_sp: PickSp} : forall s k t m l mc post1,
-      exec s k t m l mc post1 ->
-      forall post2: _ -> _ -> _ -> _ -> _ -> Prop,
-        (forall k' t' m' l' mc', post1 k' t' m' l' mc' -> post2 k' t' m' l' mc') ->
-        exec s k t m l mc post2.
+  Lemma weaken {pick_sp: PickSp} : forall s q aep k t m l mc post1,
+      exec s q aep k t m l mc post1 ->
+      forall post2: _ -> _ -> _ -> _ -> _ -> _ -> _ -> Prop,
+        (forall q' aep' k' t' m' l' mc', post1 q' aep' k' t' m' l' mc' -> post2 q' aep' k' t' m' l' mc') ->
+        exec s q aep k t m l mc post2.
   Proof.
     induction 1; intros; try solve [econstructor; eauto].
     - eapply stackalloc. 1: assumption.
@@ -193,75 +207,75 @@ Module exec. Section WithParams.
       eauto 10.
   Qed.
 
-  Lemma intersect {pick_sp: PickSp} : forall k t l m mc s post1,
-      exec s k t m l mc post1 ->
-      forall post2,
-        exec s k t m l mc post2 ->
-        exec s k t m l mc (fun k' t' m' l' mc' => post1 k' t' m' l' mc' /\ post2 k' t' m' l' mc').
-  Proof.
-    induction 1;
-      intros;
-      match goal with
-      | H: exec _ _ _ _ _ _ _ |- _ => inversion H; subst; clear H
-      end;
-      repeat match goal with
-      | H1: ?e = Some (?x1, ?y1, ?z1), H2: ?e = Some (?x2, ?y2, ?z2) |- _ =>
-        replace x2 with x1 in * by congruence;
-          replace y2 with y1 in * by congruence;
-          replace z2 with z1 in * by congruence;
-          clear x2 y2 z2 H2
-      end;
-      repeat match goal with
-             | H1: ?e = Some ?v1, H2: ?e = Some ?v2 |- _ =>
-               replace v2 with v1 in * by congruence; clear H2
-             end;
-      try solve [econstructor; eauto | exfalso; congruence].
+  (* Lemma intersect {pick_sp: PickSp} : forall q aep k t l m mc s post1, *)
+  (*     exec s q aep k t m l mc post1 -> *)
+  (*     forall post2, *)
+  (*       exec s q aep k t m l mc post2 -> *)
+  (*       exec s q aep k t m l mc (fun q' aep' k' t' m' l' mc' => post1 q' aep' k' t' m' l' mc' /\ post2 q' aep' k' t' m' l' mc'). *)
+  (* Proof. *)
+  (*   induction 1; *)
+  (*     intros; *)
+  (*     match goal with *)
+  (*     | H: exec _ _ _ _ _ _ _ |- _ => inversion H; subst; clear H *)
+  (*     end; *)
+  (*     repeat match goal with *)
+  (*     | H1: ?e = Some (?x1, ?y1, ?z1), H2: ?e = Some (?x2, ?y2, ?z2) |- _ => *)
+  (*       replace x2 with x1 in * by congruence; *)
+  (*         replace y2 with y1 in * by congruence; *)
+  (*         replace z2 with z1 in * by congruence; *)
+  (*         clear x2 y2 z2 H2 *)
+  (*     end; *)
+  (*     repeat match goal with *)
+  (*            | H1: ?e = Some ?v1, H2: ?e = Some ?v2 |- _ => *)
+  (*              replace v2 with v1 in * by congruence; clear H2 *)
+  (*            end; *)
+  (*     try solve [econstructor; eauto | exfalso; congruence]. *)
 
-    - econstructor. 1: eassumption.
-      intros.
-      rename H0 into Ex1, H13 into Ex2.
-      eapply weaken. 1: eapply H1. 1,2: eassumption.
-      1: eapply Ex2. 1,2: eassumption.
-      cbv beta.
-      intros. fwd.
-      lazymatch goal with
-      | A: map.split _ _ _, B: map.split _ _ _ |- _ =>
-        specialize @map.split_diff with (4 := A) (5 := B) as P
-      end.
-      edestruct P; try typeclasses eauto. 2: subst; eauto 10.
-      eapply anybytes_unique_domain; eassumption.
-    - econstructor.
-      + eapply IHexec. exact H5. (* not H *)
-      + simpl. intros *. intros [? ?]. eauto.
-    - eapply while_true. 1, 2: eassumption.
-      + eapply IHexec. exact H9. (* not H1 *)
-      + simpl. intros *. intros [? ?]. eauto.
-    - eapply call. 1, 2, 3: eassumption.
-      + eapply IHexec. exact H17. (* not H2 *)
-      + simpl. intros *. intros [? ?].
-        edestruct H3 as (? & ? & ? & ? & ?); [eassumption|].
-        edestruct H18 as (? & ? & ? & ? & ?); [eassumption|].
-        repeat match goal with
-               | H1: ?e = Some ?v1, H2: ?e = Some ?v2 |- _ =>
-                 replace v2 with v1 in * by congruence; clear H2
-               end.
-        eauto 10.
-    - pose proof ext_spec.mGive_unique as P.
-      specialize P with (1 := H) (2 := H7) (3 := H1) (4 := H15).
-      subst mGive0.
-      destruct (map.split_diff (map.same_domain_refl mGive) H H7) as (? & _).
-      subst mKeep0.
-      eapply interact. 1,2: eassumption.
-      + eapply ext_spec.intersect; [ exact H1 | exact H15 ].
-      + simpl. intros *. intros [? ?].
-        edestruct H2 as (? & ? & ?); [eassumption|].
-        edestruct H16 as (? & ? & ?); [eassumption|].
-        repeat match goal with
-               | H1: ?e = Some ?v1, H2: ?e = Some ?v2 |- _ =>
-                 replace v2 with v1 in * by congruence; clear H2
-               end.
-        eauto 10.
-  Qed.
+  (*   - econstructor. 1: eassumption. *)
+  (*     intros. *)
+  (*     rename H0 into Ex1, H13 into Ex2. *)
+  (*     eapply weaken. 1: eapply H1. 1,2: eassumption. *)
+  (*     1: eapply Ex2. 1,2: eassumption. *)
+  (*     cbv beta. *)
+  (*     intros. fwd. *)
+  (*     lazymatch goal with *)
+  (*     | A: map.split _ _ _, B: map.split _ _ _ |- _ => *)
+  (*       specialize @map.split_diff with (4 := A) (5 := B) as P *)
+  (*     end. *)
+  (*     edestruct P; try typeclasses eauto. 2: subst; eauto 10. *)
+  (*     eapply anybytes_unique_domain; eassumption. *)
+  (*   - econstructor. *)
+  (*     + eapply IHexec. exact H5. (* not H *) *)
+  (*     + simpl. intros *. intros [? ?]. eauto. *)
+  (*   - eapply while_true. 1, 2: eassumption. *)
+  (*     + eapply IHexec. exact H9. (* not H1 *) *)
+  (*     + simpl. intros *. intros [? ?]. eauto. *)
+  (*   - eapply call. 1, 2, 3: eassumption. *)
+  (*     + eapply IHexec. exact H17. (* not H2 *) *)
+  (*     + simpl. intros *. intros [? ?]. *)
+  (*       edestruct H3 as (? & ? & ? & ? & ?); [eassumption|]. *)
+  (*       edestruct H18 as (? & ? & ? & ? & ?); [eassumption|]. *)
+  (*       repeat match goal with *)
+  (*              | H1: ?e = Some ?v1, H2: ?e = Some ?v2 |- _ => *)
+  (*                replace v2 with v1 in * by congruence; clear H2 *)
+  (*              end. *)
+  (*       eauto 10. *)
+  (*   - pose proof ext_spec.mGive_unique as P. *)
+  (*     specialize P with (1 := H) (2 := H7) (3 := H1) (4 := H15). *)
+  (*     subst mGive0. *)
+  (*     destruct (map.split_diff (map.same_domain_refl mGive) H H7) as (? & _). *)
+  (*     subst mKeep0. *)
+  (*     eapply interact. 1,2: eassumption. *)
+  (*     + eapply ext_spec.intersect; [ exact H1 | exact H15 ]. *)
+  (*     + simpl. intros *. intros [? ?]. *)
+  (*       edestruct H2 as (? & ? & ?); [eassumption|]. *)
+  (*       edestruct H16 as (? & ? & ?); [eassumption|]. *)
+  (*       repeat match goal with *)
+  (*              | H1: ?e = Some ?v1, H2: ?e = Some ?v2 |- _ => *)
+  (*                replace v2 with v1 in * by congruence; clear H2 *)
+  (*              end. *)
+  (*       eauto 10. *)
+  (* Qed. *)
 
   Lemma eval_expr_extends_trace :
     forall e0 m l mc k v mc' k',
@@ -381,9 +395,9 @@ Module exec. Section WithParams.
           apply eval_call_args_extends_trace in H; destruct H; subst
         end.
 
-  Lemma exec_extends_trace {pick_sp: PickSp} s k t m l mc post :
-    exec s k t m l mc post ->
-    exec s k t m l mc (fun k' t' m' l' mc' => post k' t' m' l' mc' /\ exists k'', k' = k'' ++ k).
+  Lemma exec_extends_trace {pick_sp: PickSp} s q aep k t m l mc post :
+    exec s q aep k t m l mc post ->
+    exec s q aep k t m l mc (fun q' aep' k' t' m' l' mc' => post q' aep' k' t' m' l' mc' /\ exists k'', k' = k'' ++ k).
   Proof.
     intros H. induction H; try (econstructor; intuition eauto; subst_exprs; eexists; align_trace; fail).
     - econstructor; intuition eauto. intros. eapply weaken. 1: eapply H1; eauto.
@@ -403,11 +417,11 @@ Module exec. Section WithParams.
       eexists. intuition eauto. subst_exprs. eexists. align_trace.
   Qed.
 
-  Lemma exec_ext (pick_sp1: PickSp) s k t m l mc post :
-    exec (pick_sp := pick_sp1) s k t m l mc post ->
+  Lemma exec_ext (pick_sp1: PickSp) s q aep k t m l mc post :
+    exec (pick_sp := pick_sp1) s q aep k t m l mc post ->
     forall pick_sp2,
     (forall k', pick_sp1 (k' ++ k) = pick_sp2 (k' ++ k)) ->
-    exec (pick_sp := pick_sp2) s k t m l mc post.
+    exec (pick_sp := pick_sp2) s q aep k t m l mc post.
   Proof.
     intros H1 pick_sp2. induction H1; intros; try solve [econstructor; eauto].
     - econstructor; eauto. intros. replace (pick_sp1 k) with (pick_sp2 k) in *.
@@ -442,13 +456,13 @@ Module exec. Section WithParams.
     repeat (rewrite rev_app_distr || cbn [rev app] || rewrite rev_involutive);
     repeat rewrite <- app_assoc; reflexivity.
 
-  Lemma exec_to_other_trace (pick_sp: PickSp) s k1 k2 t m l mc post :
-    exec s k1 t m l mc post ->
+  Lemma exec_to_other_trace (pick_sp: PickSp) s q aep k1 k2 t m l mc post :
+    exec s q aep k1 t m l mc post ->
     exec (pick_sp := fun k => pick_sp (rev (skipn (length k2) (rev k)) ++ k1))
-      s k2 t m l mc (fun k2' t' m' l' mc' =>
-                       exists k'',
-                         k2' = k'' ++ k2 /\
-                           post (k'' ++ k1) t' m' l' mc').
+      s q aep k2 t m l mc (fun q' aep' k2' t' m' l' mc' =>
+                             exists k'',
+                               k2' = k'' ++ k2 /\
+                                 post q' aep' (k'' ++ k1) t' m' l' mc').
   Proof.
     intros H. generalize dependent k2. induction H; intros.
     - econstructor. exists nil. eauto.
@@ -503,15 +517,18 @@ Module exec. Section WithParams.
     - apply call_args_to_other_trace in H0. fwd. econstructor; intuition eauto.
       apply H2 in H0. fwd. exists l'. intuition. eexists (_ :: _).
       intuition.
+    - econstructor; eauto. exists nil. auto.
+    - apply exec_A. eauto.
+    - eapply exec_E. eauto.     
   Qed.
 
   End WithEnv.
 
   Lemma extend_env {pick_sp: PickSp} : forall e1 e2,
       map.extends e2 e1 ->
-      forall c k t m l mc post,
-      exec e1 c k t m l mc post ->
-      exec e2 c k t m l mc post.
+      forall c q aep k t m l mc post,
+      exec e1 c q aep k t m l mc post ->
+      exec e2 c q aep k t m l mc post.
   Proof. induction 2; try solve [econstructor; eauto]. Qed.
 
   End WithParams.
@@ -524,18 +541,18 @@ Section WithParams.
 
   Implicit Types (l: locals) (m: mem).
 
-  Definition call e fname k t m args mc post :=
+  Definition call e fname q aep k t m args mc post :=
     exists argnames retnames body,
       map.get e fname = Some (argnames, retnames, body) /\
       exists l, map.of_list_zip argnames args = Some l /\
-        exec e body k t m l mc (fun k' t' m' l' mc' => exists rets,
+        exec e body q aep k t m l mc (fun q' aep' k' t' m' l' mc' => exists rets,
           map.getmany_of_list l' retnames = Some rets /\ post k' t' m' rets mc').
 
-  Lemma weaken_call: forall e fname k t m args mc post1,
-      call e fname k t m args mc post1 ->
+  Lemma weaken_call: forall e fname q aep k t m args mc post1,
+      call e fname q aep k t m args mc post1 ->
       forall (post2: leakage -> trace -> mem -> list word -> MetricLog -> Prop),
       (forall k' t' m' rets mc', post1 k' t' m' rets mc' -> post2 k' t' m' rets mc') ->
-      call e fname k t m args mc post2.
+      call e fname q aep k t m args mc post2.
   Proof.
     unfold call. intros. fwd.
     do 4 eexists. 1: eassumption.
@@ -546,9 +563,9 @@ Section WithParams.
 
   Lemma extend_env_call: forall e1 e2,
       map.extends e2 e1 ->
-      forall f k t m rets mc post,
-      call e1 f k t m rets mc post ->
-      call e2 f k t m rets mc post.
+      forall f q aep k t m rets mc post,
+      call e1 f q aep k t m rets mc post ->
+      call e2 f q aep k t m rets mc post.
   Proof.
     unfold call. intros. fwd. repeat eexists.
     - eapply H. eassumption.
